apc/NormITree.v
@@ -1,4 +1,5 @@
 Require Import CRIS.
+Require Import wsim.
   
 (* Lemma isim_congruence f fl fr Ist tid is_closed r g {Rs Rt} RR ps pt nths st_src st_tgt s0 s1 t0 t1
   (EQS: s0 = s1)
@@ -24,6 +25,44 @@ Proof.
   subst. eauto.
 Qed.
 
+Lemma wsim_congruence_tgt `{!invG α Σ Γ, !subG Γ Σ, !sinvG Σ Γ α β τ}
+  f fl fr Ist u0 u1 cP is_closed r g Rs Rt RR ps pt nths sti_src st_tgt t0 t1
+  (EQ: t0 = t1):
+  f (wsim fl fr Ist is_closed u0 u1 cP r g Rs Rt RR ps pt nths sti_src (st_tgt, t0) ) ->
+  (f (wsim fl fr Ist is_closed u0 u1 cP r g Rs Rt RR ps pt nths sti_src (st_tgt, t1) ): Prop).
+Proof.
+  subst. eauto.
+Qed.
+
+Lemma wsim_congruence_src `{!invG α Σ Γ, !subG Γ Σ, !sinvG Σ Γ α β τ}
+  f fl fr Ist u0 u1 cP is_closed r g Rs Rt RR ps pt nths st_src sti_tgt t0 t1
+  (EQ: t0 = t1):
+  f (wsim fl fr Ist is_closed u0 u1 cP r g Rs Rt RR ps pt nths (st_src, t0) sti_tgt) ->
+  (f (wsim fl fr Ist is_closed u0 u1 cP r g Rs Rt RR ps pt nths (st_src, t1) sti_tgt): Prop).
+Proof.
+  subst. eauto.
+Qed.
+
+Lemma wsim_bind `{!invG α Σ Γ, !subG Γ Σ, !sinvG Σ Γ α β τ}
+  fl fr Ist is_closed u0 u1 cP r g ps pt {Rs Rt Qs Qt} RR QQ nths st_src st_tgt i_src i_tgt k_src k_tgt :
+  wsim fl fr Ist None u0 u1 cP r g Qs Qt QQ ps pt nths (st_src, i_src) (st_tgt, i_tgt)
+  ∗ (∀ nths0 st_src0 ret_src st_tgt0 ret_tgt,
+      QQ nths0 (st_src0, ret_src) (st_tgt0, ret_tgt)
+      -∗ wsim fl fr Ist is_closed u0 u1 cP r g Rs Rt RR false false nths0 (st_src0, k_src ret_src) (st_tgt0, k_tgt ret_tgt))%I
+  ⊢ (wsim fl fr Ist is_closed u0 u1 cP r g Rs Rt RR ps pt nths (st_src, i_src >>= k_src) (st_tgt, i_tgt >>= k_tgt)).
+Proof.
+  rewrite wsim.wsim_eq /wsim.wsim_def /wsim.wsim_pre. des_ifs.
+  { iIntros "[W SIM] INV". iApply isim_bind.
+    iSplitL "W". { iApply "W"; eauto. }
+    iIntros (? ? ? ? ?) "Q". iApply ("SIM" with "Q"). iFrame. }
+  { iIntros "[W SIM] INV". iApply isim_bind.
+    iSplitL "W". { iApply "W"; eauto. }
+    iIntros (? ? ? ? ?) "Q". iApply ("SIM" with "Q"). iFrame. }
+  { iIntros "[W SIM] INV". iApply isim_bind.
+    iSplitL "W". { iApply "W"; eauto. }
+    iIntros (? ? ? ? ?) "Q". iApply ("SIM" with "Q"). iFrame. }
+Qed.
+
 Lemma bind_equal {E : Type → Type} {T U : Type} t0 k0 t1 k1:
   t0 = t1 → k0 = k1 → @ITree.bind E T U t0 k0 = @ITree.bind E T U t1 k1.
 Proof.
@@ -47,5 +86,19 @@ Ltac bind_expand_l :=
   hide_itree_r;
   rewrite ?SRed.bind ?SBRed.bind ?bind_bind;
   eapply isim_congruence_src;
+  _bind_expand;
+  show_itree.
+
+Ltac wbind_expand_r := 
+  hide_itree_l;
+  rewrite ?PRed.bind ?HRed.bind ?bind_bind;
+  eapply wsim_congruence_tgt;
+  _bind_expand;
+  show_itree.
+
+Ltac wbind_expand_l := 
+  hide_itree_r;
+  rewrite ?SRed.bind ?HRed.bind ?bind_bind;
+  eapply wsim_congruence_src;
   _bind_expand;
   show_itree.
